TargetSFI/CSTest.v
@@ -1,0 +1,32 @@
+Require Import TargetSFI.CS.
+
+Import CS.
+
+
+  (* Definition eval_step_complete : Prop := *)
+  (*   forall (G : Env.t)  (st : MachineState.t) (t : trace) (st' : MachineState.t), *)
+  (*     (step G st t st') -> (eval_step G st = Some (t, st')). *)
+
+(*
+What do I need to generate?
+- G - global environment 
+   (CN,E)
+   CN - list of Component.id
+   E - list of pairs (address,Procedure.id) where 
+       address is the target of a Jal instruction 
+       that is the compilation of a Call
+- st current state
+  mem
+    mem[pc] = Instr ...
+  pc address in mem 
+  registers list of integers
+   
+- t trace 
+
+- st' next state
+ *)
+(* I need the Prop to be decidable. *)
+
+(* QuickChick eval_step_complete. *)
+                                   
+  
